investigations/cava2/Types.v
@@ -14,10 +14,15 @@
 (* limitations under the License.                                           *)
 (****************************************************************************)
 
+Require Import Lia.
+
 Require Import Coq.Arith.PeanoNat.
 Require Import Coq.Numbers.DecimalString.
 Require Import Coq.NArith.NArith.
 Require Import Coq.Strings.String.
+Require Import Coq.Lists.List.
+
+Require Import Cava.Util.Vector.
 
 Inductive type :=
 | Unit : type
@@ -27,7 +32,88 @@ Inductive type :=
 | Pair : type -> type -> type
 .
 
+Notation BitVec n := (Vec Bit n).
+
+Definition eq_dec_type (x y: type): {x = y} + {x <> y}.
+Proof.
+  decide equality.
+  apply Nat.eq_dec.
+Defined.
+
+Section RefinedLists.
+  Import ListNotations.
+
+  Notation rlist A n := {l : list A | Datatypes.length l = n}.
+
+  (* Do these exist somewhere *)
+  Lemma empty_list_with_Sn_length_is_false
+       : forall {t : Type} {n : nat} {x : list t},
+         Datatypes.length x = S n -> x = [] -> False.
+  Proof. intros; rewrite H0 in H; inversion H. Qed.
+
+  Lemma append_push_list_length
+       : forall {t : Type} {n : nat} {x0 : list t},
+         Datatypes.length x0 = S n ->
+         forall (x : t) (xs : list t), x0 = x :: xs -> Datatypes.length xs = n.
+  Proof. intros; rewrite H0 in H; cbn in *; congruence. Qed.
+
+  Definition hd_safe {t n} (ls: rlist t (S n)): (t * rlist t n) :=
+    let (ls', Hlen) := ls in
+    match ls' as ls'' return ls' = ls'' -> (t * rlist _ _) with
+    | [] => fun Heq => False_rect _ (empty_list_with_Sn_length_is_false Hlen Heq)
+    | x::xs => fun Heq => (x, exist _ xs (append_push_list_length Hlen x _ Heq))
+    end eq_refl.
+
+  Program Definition map {A B n} (f: A -> B) (ls: rlist A n): rlist B n :=
+    let (ls', Hlen) := ls in List.map f ls'.
+  Next Obligation.  rewrite map_length; reflexivity. Qed.
+
+  (* Lemma _ (tl ls : rlist A (n - 1)) _)) _ *)
+
+  Fixpoint ldrop {A} n (ls: list A): list A :=
+    match n with
+    | O => ls
+    | S n' => ldrop n' (tl ls)
+    end.
+
+  Program Fixpoint drop {A n} (m: nat) (ls: rlist A n) {struct m}: rlist A (n - m) :=
+    ldrop m ls.
+  Next Obligation.
+    revert m.
+
+    induction ls.
+    induction m.
+    - reflexivity.
+    - apply IHm.
+    - induction m; [reflexivity| apply IHls].
+  Qed.
+
+  Definition slice {A n} (start len: nat)
+      (ls: {l : list A | Datatypes.length l = n}):
+      if len <=? n - start then {l : list A | Datatypes.length l = len}
+      else unit :=
+    let (ls', Hlen) := ls in
+    if len <=? n - start then _ (drop start ls)
+    else tt.
+End.
+
+End RefinedLists.
+
 Fixpoint denote_type (t: type) :=
+  match t with
+  | Unit => unit
+  | Bit => bool
+  | Nat => nat
+    (* Experience suggests to avoid vectors? What about refined lists - will the
+    * prop size grow and be an issue with proof? *)
+    (* One pro: Prop erasure in extraction means extracted terms are smaller
+     * than vecs *)
+  | Vec t n => {l: list (denote_type t) | List.length l = n}
+  | Pair x y => (denote_type x * denote_type y)%type
+  end.
+
+(* *)
+Fixpoint denote1_type (t: type) :=
   match t with
   | Unit => unit
   | Bit => bool
@@ -35,9 +121,25 @@ Fixpoint denote_type (t: type) :=
   | Vec t n =>
     match t with
     | Bit => N
-    | _ => list (denote_type t)
+    | _ => {l: list (denote1_type t) | List.length l = n}
     end
-  | Pair x y => (denote_type x * denote_type y)%type
+  | Pair x y => (denote1_type x * denote1_type y)%type
+  end.
+
+Fixpoint denote1_to_denote {t} : denote1_type t -> denote_type t :=
+  match t return denote1_type t -> denote_type t with
+  | Vec t n =>
+    let f := denote1_to_denote in
+    match t as t1
+      return ((denote1_type t1 -> denote_type t1)
+              -> denote1_type (Vec t1 n) -> denote_type (Vec t1 n))
+    with
+    | Bit => fun _ x =>
+      let v := N2Bv_sized n x in exist _ (Vector.to_list v) (to_list_length v)
+    | _ => fun f x => map f x
+    end f
+  | Pair x y => fun '(x,y) => (denote1_to_denote x, denote1_to_denote y)
+  | _ => id
   end.
 
 Definition absorb_any (x y: type) :=
@@ -47,12 +149,36 @@ Definition absorb_any (x y: type) :=
   | _, _ => Pair x y
   end.
 
+Fixpoint ntuple t n : type :=
+  match n with
+  | O => t
+  | S n => Pair t (ntuple t n)
+  end.
+
+Definition vector_head {t n}: denote_type (Vec t (S n)) -> denote_type t * denote_type (Vec t n) := hd_safe.
+
+Fixpoint vector_as_tuple n t {struct n}: denote_type (Vec t (S n)) -> denote_type (ntuple t n) :=
+  match n with
+  | O => fun x => fst (vector_head x)
+  | S n' => fun ls =>
+    let '(hd,tl) := vector_head ls in
+    (hd, vector_as_tuple n' _ tl)
+  end.
+Definition vector_as_tuple1 n t (x: denote1_type (Vec t (S n))): denote_type (ntuple t n) :=
+  vector_as_tuple _ _ (denote1_to_denote x).
+
+Section test.
+  Import ListNotations.
+  Compute (vector_as_tuple1 _ _ (exist _ [0;1;2] _:denote1_type (Vec (BitVec 3) 3)))%N.
+  Compute (vector_as_tuple1 _ _ (exist _ [0;1;2] _:denote1_type (Vec (BitVec 3) 3)))%N.
+End test.
+
 Declare Scope circuit_type_scope.
 Delimit Scope circuit_type_scope with circuit_type.
 Open Scope circuit_type_scope.
-Notation "[ ]" := Unit (format "[ ]") : circuit_type_scope.
-Notation "[ x ]" := (Pair x Unit) : circuit_type_scope.
-Notation "[ x ; y ; .. ; z ]" := (Pair x (Pair y .. (Pair z Unit) ..)) : circuit_type_scope.
-Notation "x ** y" := (Pair x y)(at level 60, right associativity) : circuit_type_scope.
+Notation "[ ]" := unit (format "[ ]") : circuit_type_scope.
+Notation "[ x ]" := (pair x unit) : circuit_type_scope.
+Notation "[ x ; y ; .. ; z ]" := (pair x (pair y .. (pair z unit) ..)) : circuit_type_scope.
+Notation "x ** y" := (pair x y)(at level 60, right associativity) : circuit_type_scope.
 Notation "x ++ y" := (absorb_any x y) (at level 60, right associativity): circuit_type_scope.
 
